Add initial disk to Sigma state
Will use it to appropriately specify the global invariant for readers
(namely that the cache rep can hold for either the initial or current
disk, which won't matter when we get around to reading).

src/CCLProg.v
@@ -46,26 +46,30 @@ Notation heappred := (@pred ident Nat.eq_dec Var).
 
 (* The states a program steps through. *)
 Inductive Sigma :=
-| state (d:DISK) (m:heap) (hm:hashmap) (l:LockState).
+| state (d_i: DISK) (d:DISK) (m:heap) (hm:hashmap) (l:LockState).
 
 Module Sigma.
+  Definition init_disk (sigma:Sigma) :=
+    let (d_i, _, _, _, _) := sigma in d_i.
   Definition disk (sigma:Sigma) :=
-    let (d, _, _, _) := sigma in d.
+    let (_, d, _, _, _) := sigma in d.
   Definition mem (sigma:Sigma) : heap :=
-    let (_, m, _, _) := sigma in m.
+    let (_, _, m, _, _) := sigma in m.
   Definition hm (sigma:Sigma) :=
-    let (_, _, hm, _) := sigma in hm.
+    let (_, _, _, hm, _) := sigma in hm.
   Definition l (sigma:Sigma) :=
-    let (_, _, _, l) := sigma in l.
+    let (_, _, _, _, l) := sigma in l.
 
+  Definition set_init_disk (sigma:Sigma) (d_i:DISK) :=
+    let (_, d, m, hm, l) := sigma in state d_i d m hm l.
   Definition set_mem (sigma:Sigma) (m:heap) :=
-    let (d, _, hm, l) := sigma in state d m hm l.
+    let (d_i, d, _, hm, l) := sigma in state d_i d m hm l.
   Definition upd_disk (sigma:Sigma) (d':DISK -> DISK) :=
-    let (d, m, hm, l) := sigma in state (d' d) m hm l.
+    let (d_i, d, m, hm, l) := sigma in state d_i (d' d) m hm l.
   Definition upd_hm (sigma:Sigma) sz (buf: word sz) :=
-    let (d, m, hm, l) := sigma in state d m (upd_hashmap' hm (hash_fwd buf) buf) l.
+    let (d_i, d, m, hm, l) := sigma in state d_i d m (upd_hashmap' hm (hash_fwd buf) buf) l.
   Definition set_l (sigma:Sigma) l :=
-    let (d, m, hm, _) := sigma in state d m hm l.
+    let (d_i, d, m, hm, _) := sigma in state d_i d m hm l.
 End Sigma.
 
 Section CCL.
@@ -211,9 +215,6 @@ Section CCL.
                         then NonDet (* still need to check type *)
                         else Fails
                       else Fails
-    (* TODO: disk operations require guarantee proofs, too, but somehow
-    separable from memory protocol (disk operations not observable until
-    unlock, while writes are immediately visible) *)
     | BeginRead a => if CanWrite (Sigma.l sigma) then
                       match Sigma.disk sigma a with
                       | Some (v, NoReader) =>
@@ -239,19 +240,13 @@ Section CCL.
                        match l, l' with
                        | Free, Free => Fails
                        | Free, WriteLock => NonDet
-                       | WriteLock, Free => StepTo (Sigma.set_l sigma Free) tt
+                       | WriteLock, Free => NonDet (* requires guarantee proof *)
                        | WriteLock, WriteLock => Fails
                        end
                      else Fails
     | Ret v => StepTo sigma v
     | _ => NonDet
     end.
-
-  Inductive outcome T :=
-  | Finished (sigma:Sigma) (r:T)
-  | Error.
-
-  Arguments Error {T}.
 
   Inductive rtxn_step : forall T (txn:read_transaction T), heap -> T -> Prop :=
   | rtxn_step_done : forall h, rtxn_step RDone h tt
@@ -296,6 +291,18 @@ Section CCL.
       wtxn_step tid txn (upd h i (absMem (f tid m0))) h'' ->
       wtxn_step tid (WCons (AbsMemUpd i f) txn) h h''.
 
+  Inductive outcome T :=
+  | Finished (sigma:Sigma) (r:T)
+  | Error.
+
+  Arguments Error {T}.
+
+  Inductive guarantee_exec tid sigma sigma' T (v: T) : outcome T -> Prop :=
+  | GuaranteeMet : Guarantee tid sigma sigma' ->
+                   guarantee_exec tid sigma sigma' v (Finished sigma' v)
+  | GuaranteeNotMet : ~Guarantee tid sigma sigma' ->
+                      guarantee_exec tid sigma sigma' v Error.
+
   Inductive exec (tid:TID) : forall T, Sigma -> cprog T -> outcome T -> Prop :=
   | ExecStepDec : forall T (p: cprog T) sigma sigma' v,
       step_dec sigma p = StepTo sigma' v ->
@@ -308,58 +315,58 @@ Section CCL.
       hash_safe (Sigma.hm sigma) h buf ->
       exec tid sigma (@Hash sz buf) (Finished (Sigma.upd_hm sigma buf) h)
   | ExecBindFinish : forall T T' (p: cprog T') (p': T' -> cprog T)
-                       sigma sigma' v out,
-      exec tid sigma p (Finished sigma' v) ->
-      exec tid sigma' (p' v) out ->
-      exec tid sigma (Bind p p') out
-  | ExecBindFail : forall T T' (p: cprog T') (p': T' -> cprog T) sigma,
-      exec tid sigma p Error ->
-      exec tid sigma (Bind p p') Error
+                       st st' v out,
+      exec tid st p (Finished st' v) ->
+      exec tid st' (p' v) out ->
+      exec tid st (Bind p p') out
+  | ExecBindFail : forall T T' (p: cprog T') (p': T' -> cprog T) st,
+      exec tid st p Error ->
+      exec tid st (Bind p p') Error
   | ExecWriteLock : forall sigma sigma',
       Sigma.l sigma = Free ->
       Rely tid sigma sigma' ->
       hashmap_le (Sigma.hm sigma) (Sigma.hm sigma') ->
+      Sigma.init_disk sigma' = Sigma.disk sigma' ->
       let sigma' := Sigma.set_l sigma' WriteLock in
       exec tid sigma (SetLock Free WriteLock) (Finished sigma' tt)
+  | ExecUnlock : forall sigma out,
+      Sigma.l sigma = WriteLock ->
+      let sigma' := Sigma.set_l (Sigma.set_init_disk sigma (Sigma.disk sigma)) Free in
+      guarantee_exec tid sigma sigma' tt out ->
+      exec tid sigma (SetLock WriteLock Free) out
   | ExecAlloc : forall sigma A (v:A) i,
       Sigma.mem sigma i = None ->
       let sigma' := Sigma.set_mem sigma (upd (Sigma.mem sigma) i (val v)) in
-      exec tid sigma (Alloc v)
-           (Finished sigma' i)
+      exec tid sigma (Alloc v) (Finished sigma' i)
   | ExecReadTxn : forall sigma A (txn:read_transaction A) v sigma',
       rtxn_step txn (Sigma.mem sigma) v ->
       (Sigma.l sigma = WriteLock -> sigma' = sigma) ->
       (Sigma.l sigma = Free -> Rely tid sigma sigma' /\
                       hashmap_le (Sigma.hm sigma) (Sigma.hm sigma') /\
+                      Sigma.init_disk sigma' = Sigma.disk sigma' /\
                       Sigma.l sigma' = Sigma.l sigma) ->
       exec tid sigma (ReadTxn txn)
            (Finished sigma' v)
   | ExecReadTxnFail : forall sigma A (txn:read_transaction A),
       rtxn_error txn (Sigma.mem sigma) ->
       exec tid sigma (ReadTxn txn) Error
-  | ExecAssgnTxn : forall sigma (txn:write_transaction) h',
+  | ExecAssgnTxn : forall sigma (txn:write_transaction) h' out,
       Sigma.l sigma = WriteLock ->
       wtxn_step tid txn (Sigma.mem sigma) h' ->
       let sigma' := Sigma.set_mem sigma h' in
-      Guarantee tid sigma sigma' ->
-      exec tid sigma (AssgnTxn txn)
-           (Finished sigma' tt)
-  | ExecAssgnTxnProtocolError : forall sigma (txn:write_transaction) h',
-      Sigma.l sigma = WriteLock ->
-      wtxn_step tid txn (Sigma.mem sigma) h' ->
-      let sigma' := Sigma.set_mem sigma h' in
-      ~Guarantee tid sigma sigma' ->
-      exec tid sigma (AssgnTxn txn) Error
+      guarantee_exec tid sigma sigma' tt out ->
+      exec tid sigma (AssgnTxn txn) out
   | ExecAssgnTxnTyError : forall sigma (txn:write_transaction),
       wtxn_error txn (Sigma.mem sigma) ->
       exec tid sigma (AssgnTxn txn) Error.
 
-  Theorem ExecRet : forall tid T (v:T) sigma,
-      exec tid sigma (Ret v) (Finished sigma v).
+  Theorem ExecRet : forall tid T (v:T) st,
+      exec tid st (Ret v) (Finished st v).
   Proof.
     intros.
+    destruct st.
     eapply ExecStepDec.
-    auto.
+    reflexivity.
   Qed.
 
   Definition SpecDouble T :=
@@ -422,6 +429,12 @@ Module CCLTactics.
       clear H
     end.
 
+  Ltac inv_guarantee :=
+    match goal with
+    | [ H: guarantee_exec _ _ _ _ _ _ |- _ ] =>
+      inversion H; subst; clear H
+    end.
+
   Local Ltac inv_cleanup H :=
     inversion H; subst; repeat inj_pair2.
 
@@ -437,6 +450,7 @@ Module CCLTactics.
                    let n := numgoals in guard n <= 1
                  end
         end;
+    try inv_guarantee;
     repeat match goal with
            | [ H: StepTo _ _ = StepTo _ _ |- _ ] =>
              inversion H; subst; clear H
