src/CCLHashExec.v
@@ -2,51 +2,56 @@ Require Import CCLProg.
 Require Import Hashmap.
 Require Import Automation.
 
-Theorem exec_hashmap_le : forall T (p: cprog T)
-                            G tid sigma out,
-    exec G tid sigma p out ->
-    match out with
-    | Finished sigma' _ => hashmap_le (Sigma.hm sigma) (Sigma.hm sigma')
-    | Error => True
-    end.
-Proof.
-  intros.
-  generalize dependent sigma.
-  induction 1; intros; auto;
+Section HashExec.
+
+  Hint Resolve hashmap_le_refl.
+
+  Theorem exec_hashmap_le : forall T (p: cprog T)
+                              G tid sigma out,
+      exec G tid sigma p out ->
+      match out with
+      | Finished sigma' _ => hashmap_le (Sigma.hm sigma) (Sigma.hm sigma')
+      | Error => True
+      end.
+  Proof.
+    intros.
+    generalize dependent sigma.
+    induction 1; intros; auto;
       repeat match goal with
              | [ x := _ |- _ ] => subst x
              | [ |- hashmap_le (Sigma.hm _) (Sigma.hm _) ] =>
                repeat match goal with
                       | [ sigma: Sigma |- _ ] => destruct sigma
                       end; simpl in *; reflexivity
+             | _ => progress CCLTactics.inv_guarantee
+             | _ => solve [ auto ]
              end.
-  - destruct sigma.
-    destruct p;
-      repeat match goal with
-             | [ H: context[match ?d with | _ => _ end] |- _ ] =>
-               destruct d
-             | [ H: StepTo _ _ = StepTo _ _ |- _ ] =>
-               inversion H; subst; clear H
-             | [ |- hashmap_le ?a ?a ] => reflexivity
-             | _ => progress simpl in *
-             | _ => congruence
-             end.
-  - repeat match goal with
-           | [ sigma: Sigma |- _ ] => destruct sigma; simpl in *
-           end;
-      try reflexivity;
+    - destruct sigma.
+      destruct p;
+        repeat match goal with
+               | [ H: context[match ?d with | _ => _ end] |- _ ] =>
+                 destruct d
+               | [ H: StepTo _ _ = StepTo _ _ |- _ ] =>
+                 inversion H; subst; clear H
+               | _ => progress simpl in *
+               | _ => auto; congruence
+               end.
+    - repeat match goal with
+             | [ sigma: Sigma |- _ ] => destruct sigma; simpl in *
+             end;
+        eauto.
+      unfold hashmap_le.
+      eexists.
+      econstructor; eauto.
+      constructor.
+    - destruct out; eauto.
+      etransitivity; eauto.
+    - destruct sigma'; simpl in *.
       eauto.
-    unfold hashmap_le.
-    eexists.
-    econstructor; eauto.
-    constructor.
-  - destruct out; eauto.
-    etransitivity; eauto.
-  - destruct sigma'; simpl in *.
-    eauto.
-  - destruct (Sigma.l sigma); intuition subst.
-    reflexivity.
-Qed.
+    - destruct (Sigma.l sigma); intuition (subst; eauto).
+  Qed.
+
+End HashExec.
 
 (* Local Variables: *)
 (* company-coq-local-symbols: (("Sigma" . ?Σ) ("sigma" . ?σ) ("sigma'" . (?σ (Br . Bl) ?'))) *)
